more notes on contextual equivalence

rocq/untyped/ctx.v
@@ -1,7 +1,8 @@
-From Stdlib Require Import Psatz.
-From Stdlib Require Import Arith.
+(** This file is Pitt's definition of Contextual Approximation
+    as the largest compatible, adequate, preorder 
+    for scoped relations.
+*)
 
-Require Export common.core.
 Require Export untyped.stack.
 
 Import Lists.List.ListNotations.
@@ -11,27 +12,41 @@ Import stack.Notations.
 Open Scope list_scope.
 Open Scope rec_scope.
 
-
 (* --------------------------------------------------------- *)
 
-Definition scoped_relation (T : nat -> Type) := forall n, T n -> T n -> Prop.
+(** A scoped relation is a binary relation between two objects
+    in the same scope. We make this generic so that we can use 
+    the same definition for terms and values. *)
+Definition scoped_relation (T : nat -> Type) : Type := forall n, T n -> T n -> Prop.
 
-Class Reflexive {T : nat -> Type} (R : scoped_relation T) : Prop := 
-  { scoped_refl : forall n x, R n x x }.
+(** A scoped relation is a pre-order if it is reflexive and transitive. 
+    We define type classes for these concepts, similar to the 
+    type classes found in Rocq's standard library.
+    For more background on typeclasses, see this chapter 
+    https://softwarefoundations.cis.upenn.edu/qc-current/Typeclasses.html
+ *)
+Class ScopedReflexive {T : nat -> Type} (R : scoped_relation T) : Prop := 
+  scoped_refl : forall n x, R n x x.
+Class ScopedTransitive {T : nat -> Type} (R : scoped_relation T) : Prop := 
+  scoped_trans : forall n (t1 t2 t3 : T n), R _ t1 t2 -> R _ t2 t3 -> R _ t1 t3.
 
-Class Transitive {T : nat -> Type} (R : scoped_relation T) : Prop := 
-  { scoped_trans : forall n (t1 t2 t3 : T n), R _ t1 t2 -> R _ t2 t3 -> R _ t1 t3 }.
+Arguments scoped_refl {_}{_}.
+Arguments scoped_trans {_}{_}{_}{_}.
 
-Class PreOrder {T : nat -> Type} (R : scoped_relation T) := 
-  { po_scoped_refl  : Reflexive R ;
-    po_scoped_trans : Transitive R
+Class ScopedPreOrder {T : nat -> Type} (R : scoped_relation T) := 
+  { po_scoped_refl  :: ScopedReflexive R ;
+    po_scoped_trans :: ScopedTransitive R
   }.
 
-Definition Adequate (RE : scoped_relation Tm) := 
-  forall (e e' : Tm 0), RE _ e e' -> Small.halts (nil, e) -> Small.halts (nil, e').
+(** A relation is Adequate when related *closed* values 
+    obey approximation. *)
+Class Adequate (RE : scoped_relation Tm) := 
+  adequate : forall (e e' : Tm 0), RE _ e e' -> (nil, e) ⊑ (nil, e').
 
-Existing Class Adequate.
-
+(** Compatibility is specific to the syntax of the language. It states
+    that the relation is preserved through all syntactic forms. Because 
+    our language has two mutual types (Tm and Val) we need to index 
+    compatibility by two relations, that must work together. *)
 Class Compatible (RE : scoped_relation Tm) (RV : scoped_relation Val) := 
   { val_var n x :
       RV n (var x) (var x) ;
@@ -75,22 +90,14 @@ Class Compatible (RE : scoped_relation Tm) (RV : scoped_relation Val) :=
 
 }.
 
-(** * Contextual preorder definition *)
-
-Inductive CTX n (e e' : Tm n) : Prop := 
-  rel : forall RE RV, 
-      Compatible RE RV -> 
-      Adequate RE -> 
-      Transitive RE ->
-      RE n e e' -> CTX n e e'.
-
-(** * We want to know properties about CTX *)
 
 
 (** ---------------------------------------------------- * *)
 
-(* Any relation that is compatible is also reflexive *)
+(* Any relation that is compatible is also reflexive. We prove this 
+   by (mutual) induction on the syntax of Tm and Val. *)
 
+(** Combined mutual induction scheme *)
 Scheme Val_Tm_rec := Induction for Val Sort Prop 
     with 
     Tm_Val_rec := Induction for Tm Sort Prop.
@@ -114,85 +121,117 @@ Proof.
   - eapply val_succ; eauto.
 (* FILL IN HERE *) Admitted.
 
-Instance Compatible_ReflexiveRE {RE}{RV} `{H : Compatible RE RV} : Reflexive RE.
-constructor. intro n.
-move: (Compatible_refl _ _ H) => h1.
-eapply (h1 n).
+Instance Compatible_ReflexiveRE {RE}{RV} `{H : Compatible RE RV} : ScopedReflexive RE.
+Proof.
+  intro n.
+  move: (Compatible_refl _ _ H) => h1.
+  eapply (h1 n).
 Qed.
 
-Instance Compatible_ReflexiveRV {RE RV} `{H : Compatible RE RV} : Reflexive RV.
-constructor. intro n.
-move: (Compatible_refl _ _ H) => h1.
-eapply (h1 n).
+Instance Compatible_ReflexiveRV {RE RV} `{H : Compatible RE RV} : ScopedReflexive RV.
+Proof.
+  intro n.
+  move: (Compatible_refl _ _ H) => h1.
+  eapply (h1 n).
 Qed.
 
+(** ---------------------------------------------------- * *)
 
-(* ------------------------------------------------------------------ *)
+(** * CTX: Pitt's contextual preorder *)
 
-(* We won't show that CTX is compatible here, but we can show that it 
-   is both Adequate and Transitive *)
+(** Pitt's defines contextual approximation as the largest 
+    Compatible, Adequate, PreOrder. We can model that definition 
+    by saying that any two terms are related by CTX when they 
+    are related by any Compatible, Adequate, Transitive relation 
+    (We showed above that Compatible implies reflexive so we 
+    don't need to include that in the definition.)
+    Note that RV is unconstrained --- it only needs to be 
+    compatible with RE.
+*)
+Inductive CTX n (e e' : Tm n) : Prop := 
+  rel : forall RE RV 
+      `{Compatible RE RV} 
+      `{Adequate RE} 
+      `{ScopedTransitive _ RE},
+      RE n e e' -> CTX n e e'.
+
+
+
+(* This definition shows that CTX is at least as big as any Compatible,
+   Adequate, Transitive relation, but it doesn't show that it has any of these
+   properties itself. We need to prove it.
+
+   It is difficult to show that CTX is compatible, but we will show that
+   it is both Adequate (easy) and Transitive (a little more difficult). *)
 
 (** Adequacy of CTX is straightforward *)
 
 Instance Adequate_CTX : Adequate CTX.
-unfold Adequate.
-intros e e' h1 h.
-inversion h1.
-eapply H0; eauto.
+Proof.
+  unfold Adequate.
+  intros e e' h1 h.
+  inversion h1. eapply adequate; eauto.
 Qed.
 
-(* ------------------------------------------------------------------ *)
+(** * Transtivity of CTX *)
 
-(** Transtivity of CTX is more difficult to show *)
+(* We can show that CTX is transitive by showing that the transitive 
+   closure of two Adequate, Transitive, Compatible relations is 
+   itself Adequate, Transitive and Compatible. *)
 
+(** transitive closure of RE1 + RE2 *) 
 Inductive OR_star {T : nat -> Type} (RE1 RE2: scoped_relation T) n (t1 t2 : T n) : Prop := 
-  | OR_1 : RE1 n t1 t2 -> OR_star RE1 RE2 n t1 t2 
-  | OR_2 : RE2 n t1 t2 -> OR_star RE1 RE2 n t1 t2 
+  | OR_1 : 
+    RE1 n t1 t2 -> OR_star RE1 RE2 n t1 t2 
+  | OR_2 : 
+    RE2 n t1 t2 -> OR_star RE1 RE2 n t1 t2 
   | OR_trans t3 : 
     OR_star RE1 RE2 n t1 t3
     -> OR_star RE1 RE2 n t3 t2 
     -> OR_star RE1 RE2 n t1 t2. 
 
 Instance Reflexive_OR_star {T} {RE1 RE2 : scoped_relation T} 
-  `{Reflexive T RE1} : Reflexive (OR_star RE1 RE2).
+  `{ScopedReflexive _ RE1} : ScopedReflexive (OR_star RE1 RE2).
 Proof.
-constructor.
 - intros n t.
   eapply OR_1; eapply scoped_refl; eauto.
 Qed.
 
 Instance Transitive_OR_star {T} {RE1 RE2 : scoped_relation T} :
-  Transitive (OR_star RE1 RE2).
+  ScopedTransitive (OR_star RE1 RE2).
 Proof.
-constructor.
-- intros n t1 t2 t3 O1 O2.    
+- intros n t1 t2 t3 O1 O2.
   eapply OR_trans; eauto.
 Qed.
 
 Instance PreOrder_OR_star {T} {RE1 RE2 : scoped_relation T} 
-  `{Reflexive T RE1} : 
-  PreOrder (OR_star RE1 RE2).
-split. constructor; eapply scoped_refl. constructor; eapply scoped_trans.
+  `{ScopedReflexive T RE1} : 
+  ScopedPreOrder (OR_star RE1 RE2).
+Proof.
+  split; typeclasses eauto.
 Qed.
 
 Instance Adequate_OR_star {RE1 RE2 : scoped_relation Tm} `{Adequate RE1} `{Adequate RE2} : Adequate (OR_star RE1 RE2). 
 Proof.
 unfold Adequate in *.
-intros e e' O. induction O; eauto.
+intros e e' O. induction O; eauto. transitivity ([] : stack, t3); auto.
 Qed.
 
-Ltac compat_case H1 f := 
-induction H1; [ 
-  eapply OR_1; eapply f; eauto |
-  eapply OR_2; eapply f; eauto |
-  eapply OR_trans; eauto].
-
+(* Tactic to help with compatiblility proof below. *)
+Ltac compat_case t1 t2 f := 
+match goal with [ H1 : OR_star _ _ _ t1 t2 |- _ ] => 
+                  induction H1; [ 
+                    eapply OR_1; eapply f; eauto |
+                    eapply OR_2; eapply f; eauto |
+                    eapply OR_trans; eauto] end;
+try match goal with [ |- _ _ ?t ?t ] => 
+  eapply scoped_refl; eauto using Compatible_ReflexiveRV, Compatible_ReflexiveRE end;
+eauto.
 
 Instance Compatible_OR_star 
   {RE1 RE2 : scoped_relation Tm}
   {RV1 RV2 : scoped_relation Val} 
-   `{PreOrder Tm RE1} `{PreOrder Tm RE2}
-   `{Reflexive _ RV1} `{Reflexive _ RV2}
+   `{ScopedPreOrder Tm RE1} `{ScopedPreOrder Tm RE2}
    `{Compatible RE1 RV1} `{Compatible RE2 RV2} : 
   Compatible (OR_star RE1 RE2) (OR_star RV1 RV2).      
 Proof.               
@@ -201,25 +240,19 @@ all: intros.
 - eapply OR_1; eapply val_var; eauto.
 - eapply OR_1; eapply val_unit; eauto.
 - eapply OR_1; eapply val_zero; eauto.
-- compat_case H5 @val_succ.
+- compat_case x y @val_succ.
 (* FILL IN HERE *) Admitted.
 
-Instance Transitive_CTX : Transitive CTX.
-constructor.
-- intros n t1 t2 t3 C1 C2.
+Instance Transitive_CTX : ScopedTransitive CTX.
+Proof.
+  intros n t1 t2 t3 C1 C2.
   destruct C1 as [RE1 RV1 ? ? ? R1].
   destruct C2 as [RE2 RV2 ? ? ? R2].
   eapply (rel n t1 t3 (OR_star RE1 RE2) (OR_star RV1 RV2)).
+  eapply OR_trans. eapply OR_1; eauto. eapply OR_2; eauto.
+  Unshelve.
   + eapply Compatible_OR_star; eauto.
-    Unshelve. split; eauto. 
-    constructor. eapply scoped_refl. 
-    split; eauto.
-    constructor. eapply scoped_refl.
-  + eapply Adequate_OR_star; eauto.
-  + eapply PreOrder_OR_star; eauto.
-  + eapply OR_trans. eapply OR_1; eauto.
-    eapply OR_2; eauto.
+    Unshelve. split; typeclasses eauto. 
+    split; typeclasses eauto.
 Qed.
-
-(** --------------------------------------------------------- *)
 
