rocq/untyped/stack.v
@@ -1,4 +1,5 @@
 Require Export untyped.prim.
+Require Export Classes.RelationClasses.
 
 Import SyntaxNotations.
 Import Lists.List.ListNotations.
@@ -28,18 +29,19 @@ Local Reserved Notation "m ↦ m'" (at level 70).
 Inductive step : machine -> machine -> Prop := 
   | s_prim s e e' : 
     e ~>> e' ->
-    (s , e) ↦ (s, e')
+    (s, e) ↦ (s, e')
 
   | s_pop s e2 v : 
     (f_let e2 :: s, ret v) ↦ (s, e2[v..])
 
   | s_push  s e1 e2 : 
-    (s , let_ e1 e2 ) ↦ (f_let e2 :: s, e1)
+    (s, let_ e1 e2 ) ↦ (f_let e2 :: s, e1)
 where "m ↦ m'" := (step m m') : rec_scope.
   
 Definition irreducible (m : machine) : Prop := 
   forall m', not (m ↦ m').
 
+(** Machine steps are deterministic *)
 Lemma deterministic :
   forall m m1 m2, (m ↦ m1) -> (m ↦ m2) -> m1 = m2.
 Proof.
@@ -51,16 +53,38 @@ Proof.
 Qed.
 
 
+(** The program halts in exactly n steps *)
 Definition halts_n (m : machine) n : Prop := 
   exists v, step_n step n m (nil, ret v).
 
+(** The program halts in an unspecified number of steps *)
 Definition halts (m : machine) : Prop := 
   exists v, multi step m (nil, ret v).
 
+(** An approximation relation based on halting behavior *)
+Definition approx (m1 m2 : machine) : Prop := 
+  halts m1 -> halts m2.
+
+(** A step-indexed approximation: the first machine must halt
+    within the specified number of steps. *)
+Definition approx_n m1 m2 n : Prop := 
+  halts_n m1 n -> halts m2.
+  
+End Small.
+
+Module Notations.
+Infix "↦"  := Small.step (at level 70) : rec_scope.
+Infix "↦*" := (multi Small.step) (at level 70) : rec_scope.
+Infix "⊑"  := Small.approx (at level 70) : rec_scope.
+Notation "m ⊑n m' @"  := (Small.approx_n m m') (at level 70) : rec_scope.
+End Notations.
+
+Import Notations.
+
 Lemma halts_reverse_prim s e e' : 
-  halts (s, e') ->
+  Small.halts (s, e') ->
   e ~>> e' ->
-  halts (s, e).
+  Small.halts (s, e).
 Proof.
   intros h ss.
   destruct h as [m sn].
@@ -68,38 +92,20 @@ Proof.
 Qed.
 
 Lemma halts_reverse m m' : 
-  halts m ->
+  Small.halts m ->
   m' ↦ m ->
-  halts m'.
+  Small.halts m'.
 Proof.
   intros h ss.
   destruct h as [k sn].
   exists k. econstructor; eauto. 
 Qed.
 
-End Small.
-
-Module Notations.
-Infix "↦"  := Small.step (at level 70) : rec_scope.
-Infix "↦*" := (multi Small.step) (at level 70) : rec_scope.
-End Notations.
-
-Import Notations.
-
 Lemma terminal_halts {v} : 
   Small.halts (nil, ret v).
 Proof.
   exists v. eapply ms_refl; eauto.
 Qed.
-
-Lemma halts_reverse {m m'}:
-  Small.halts m' ->  m ↦ m' ->
-  Small.halts m.
-Proof.
-  intros [v h] ss.
-  exists v. econstructor; eauto.
-Qed.
-
 
 Lemma halts_forward {m m'}:
   Small.halts m -> m ↦ m' -> 
@@ -129,4 +135,63 @@ Proof.
   exists v. econstructor; eauto.
 Qed.
 
+(** * Properties of the approximation relation *)
+
+Instance approx_refl : Reflexive Small.approx.
+Proof. unfold Small.approx. done. Qed.
+
+Instance approx_trans : Transitive Small.approx.
+Proof. unfold Small.approx. unfold Transitive. intros. eauto. Qed.
+
+Lemma approx_n_refl { m k } : m ⊑n m @ k.
+Proof.
+  unfold Small.approx_n. intro h. unfold Small.halts.
+  unfold Small.halts_n in h.
+  destruct h as [v SS].
+  eapply step_n_multi in SS.
+  eexists; eauto.
+Qed.
+
+Lemma approx_n_trans { m1 m2 m3 } : 
+  (forall k, m1 ⊑n m2 @ k) -> (forall k, m2 ⊑n m3 @ k)  -> (forall k,  m1 ⊑n m3 @ k).
+Proof.
+  unfold Small.approx_n.
+  unfold Small.halts_n.
+  unfold Small.halts.
+  intros h1 h2 k HH. 
+  move: (h1 k HH) => [v1 SS].
+  move: (multi_step_n Small.step _ _ SS) => [k2 SS2].
+  eapply (h2 k2). eexists; eauto.
+Qed.
+
+Lemma approx_forward { m1 m2 } : m1 ↦ m2 -> m1 ⊑ m2.
+unfold Small.approx. intros. eapply halts_forward; eauto. Qed.
+
+Lemma approx_forward_prim { s e1 e2 } : e1 ~>> e2 -> (s,e1) ⊑ (s, e2).
+unfold Small.approx. intros. eapply halts_forward; eauto.
+eapply Small.s_prim; eauto. Qed.
+
+Lemma approx_reverse { m1 m2 } : m1 ↦ m2 -> m2 ⊑ m1.
+unfold Small.approx. intros. eapply halts_reverse; eauto. Qed.
+
+Lemma approx_reverse_prim { s e1 e2 } : e1 ~>> e2 -> (s,e2) ⊑ (s,e1).
+unfold Small.approx. intros. eapply halts_reverse; eauto. eapply Small.s_prim; eauto. Qed.
+
+
+Lemma approx_n_forward { m1 m2 k } : m1 ↦ m2 -> m1 ⊑n m2 @ k.
+unfold Small.approx_n. intros. 
+eapply halts_n_forward in H0; eauto. destruct H0 as [j [EQ [v h0]]].
+exists v. eapply step_n_multi; eauto. Qed.
+
+Lemma approx_n_forward_prim { s e1 e2 k } : e1 ~>> e2 -> (s,e1) ⊑n (s, e2) @ k.
+intros. eapply approx_n_forward. eapply Small.s_prim; eauto. Qed.
+
+Lemma approx_n_reverse { m1 m2 k} : m1 ↦ m2 -> m2 ⊑n m1 @ k.
+unfold Small.approx_n. intros. 
+eapply halts_n_reverse in H0; eauto. destruct H0 as [v h0]. 
+exists v. eapply step_n_multi; eauto. Qed.
+
+Lemma approx_n_reverse_prim { s e1 e2 k } : e1 ~>> e2 -> (s,e2) ⊑n (s,e1) @k.
+intros. eapply approx_n_reverse; eauto. eapply Small.s_prim; eauto.
+Qed.
 
