rocq/untyped/example_equiv.v
@@ -1,0 +1,354 @@
+From Stdlib Require Import Psatz.
+From Stdlib Require Import Arith.
+
+Require Import rec.iprop.
+Require Import untyped.stack.
+
+Require Export untyped.equiv.
+Require Export untyped.contextual.
+
+Import SyntaxNotations.
+Import Lists.List.ListNotations.
+Import untyped.stack.Notations.
+Import rec.iprop.Notations.
+
+Open Scope iProp_scope.
+Open Scope list_scope.
+Open Scope rec_scope.
+
+Import FinValues.
+
+Module Notations.
+Notation "e <=CTX e'" := (CTX _ e e') (at level 70).
+Notation "e <=CTX e'" := (CTX _ e e') (at level 70).
+Notation "e <=CIU e'" := (CIU _ e e') (at level 70).
+Notation "e <=log e'" := (logtm _ e e') (at level 70).
+End Notations.
+
+Import Notations.
+
+(** * "Beta" reduction rules. *)
+
+(*  X |- (\x. e)v <= e[v/x] *)
+Lemma fun_beta n (e : Tm (S (S n))) (v : Val n) :
+  (app (abs e) v) <=CIU e[v .: (abs e)..].
+Proof.
+  intros σ s.
+  cbn.
+  intro h.
+  eapply halts_forward in h.
+  2: { eapply Small.s_prim. eapply s_beta. } 
+  asimpl in h.
+  done.
+Qed.
+
+Lemma ifz_zero_beta n (e1 : Tm n) e2 :
+  ifz zero e1 e2 <=CIU e1.
+Proof.
+  intros σ s.
+  cbn.
+  intro h.
+  eapply halts_forward in h. 
+  2: { eapply Small.s_prim. eapply s_ifz_zero. } 
+  done.
+Qed.                           
+
+Lemma ifz_succ_beta n v (e1 : Tm n) e2 :
+  ifz (succ v) e1 e2 <=CIU e2 [ v .. ] .
+Proof.
+  intros σ s.
+  cbn.
+  intro h.
+  eapply halts_forward in h. 
+  2: { eapply Small.s_prim. eapply s_ifz_succ. } 
+  asimpl in h.
+  done.
+Qed.                           
+
+Lemma let_ret n (e : Tm (S n)) v : 
+  let_ (ret v) e <=CIU e[v..].
+Proof.
+  intros σ s.
+  cbn.
+  intro h.
+  eapply halts_forward in h.
+  2: { eapply Small.s_push. } 
+  eapply halts_forward in h.
+  2: { eapply Small.s_pop. } 
+  asimpl in h.
+  done.
+Qed.
+
+
+Lemma fun_beta_expand n (e : Tm (S (S n))) (v : Val n) :
+   e[v .: (abs e)..] <=CIU (app (abs e) v).
+Proof.
+  intros σ s.
+  cbn.
+  intro h.
+  eapply halts_reverse.
+   2: { eapply Small.s_prim. eapply s_beta. } 
+  asimpl in h.
+  done.
+Qed.
+
+Lemma ifz_zero_beta_expand n (e1 : Tm n) e2 :
+  e1 <=CIU ifz zero e1 e2.
+Proof.
+ intros σ s.
+ cbn.
+ intro h.
+ eapply halts_reverse.
+ 2: { eapply Small.s_prim. eapply s_ifz_zero. } 
+ done.
+Qed.
+
+Lemma ifz_succ_beta_expand n v (e1 : Tm n) e2 :
+  e2 [ v .. ] <=CIU ifz (succ v) e1 e2.
+Proof.
+  intros σ s.
+  cbn.
+  intro h.
+  eapply halts_reverse. 
+  2: { eapply Small.s_prim. eapply s_ifz_succ. } 
+  asimpl in h.
+  done.
+Qed.                           
+
+Lemma let_ret_expand n (e : Tm (S n)) v : 
+  e[v..] <=CIU let_ (ret v) e.
+Proof.
+  intros σ s.
+  cbn.
+  intro h.
+  eapply halts_reverse.
+  2: { eapply Small.s_push. } 
+  eapply halts_reverse.
+  2: { eapply Small.s_pop. } 
+  asimpl in h.
+  done.
+Qed.
+
+
+  
+
+(** * "Eta" reduction rules. *)
+
+(*  X |- \x. v x == v *)
+(* Uses logical relation *)
+Lemma fun_eta n (v : Val n) :
+  logval n (abs (app v⟨↑⟩⟨↑⟩ (var f0))) v.
+Proof.
+  unfold logval.
+  intros k σ1 σ2 Es.
+  cbn.
+  rewrite V_def.
+  intros v1 v1' j LEj. next j.
+  intros Vvv.
+  asimpl.
+  eapply C_app.
+  have Ev: logval n v v. eapply scoped_refl. typeclasses eauto.
+  unfold logval in Ev.
+  eapply Ev. eapply dclosed; eauto. lia.
+  auto.
+Qed.
+
+
+Lemma nat_eta n (v : Val n) :
+  logtm n (ifz v (ret zero) (ret (succ (var var_zero)))) (ret v).
+Proof.
+  unfold logtm.
+  intros k σ1 σ2 Es.
+  cbn.
+  have EV: logval n v v. eapply scoped_refl. typeclasses eauto.
+  rewrite C_def.
+  intros s s' j LEj StE. 
+  rewrite St_def in StE.
+  intros [v1 h].
+  inversion h; subst; clear h.
+  inversion H; subst; clear H.
+  destruct v[σ1] eqn:EQH;
+  auto_unfold in *; rewrite EQH in H4; inversion H4; subst; clear H4.
+  - specialize (EV k0 σ1 σ2).
+    specialize (StE zero v[σ2] k0 ltac:(lia)).
+    eapply StE.
+    rewrite <- EQH.
+    eapply EV.
+    eapply dclosed; eauto.
+    lia.
+    exists v1. eauto.
+  - cbn in H0.
+    unfold logval in EV.
+    specialize (EV k _ _ Es). 
+    auto_unfold in *. rewrite EQH in EV.
+    rewrite V_def in EV. destruct v[σ2] eqn: EQH2.
+    all: auto_unfold in *; rewrite EQH2 in EV; try done.
+    eapply StE.
+    3: { exists v1. eapply H0. }  lia.
+    auto_unfold in *. rewrite EQH2.
+    rewrite V_def.
+    eapply dclosed; eauto. lia.
+Qed.
+
+(** * failure of eta-expansion rules *)
+
+
+(* The opposite is not true because we don't have types. For example 
+   v could be "0". *)
+Lemma not_fun_eta_expand :
+  not (forall (v : Val 0), ContextualVal _ v (abs (app v⟨↑⟩⟨↑⟩ (var f0)))).
+Proof.
+  intros h.
+  specialize (h zero).
+  unfold ContextualVal in h.
+  specialize (h (c_ifz1 c_hole (ret zero) (ret zero))).
+  cbn in h.
+  have PRE: Small.halts ([], ifz zero (ret zero) (ret zero)). eexists. eapply ms_trans.
+  eapply Small.s_prim. eapply s_ifz_zero. eapply ms_refl.
+  specialize (h PRE). clear PRE.
+  destruct h as [v h1].
+  inversion h1. subst. clear h1.
+  inversion H. subst. clear H.
+  inversion H4.
+Qed.
+
+(** * Beta equivalence implies contextual/oberservational equivalence. But does not relate as many terms *)
+
+Reserved Notation "t1 =β t2" (at level 70).
+Reserved Notation "t1 =vβ t2" (at level 70).
+
+Inductive BE (n : nat) : Tm n -> Tm n -> Prop :=
+  | BE_beta : forall (e : Tm _) (v : Val _), 
+      app (abs e) v =β e[v .: (abs e)..]
+  | BE_ifz_zero : forall (e1 : Tm n) (e2 : Tm (S n)), 
+      ifz zero e1 e2 =β e1
+  | BE_ifz_succ : forall (e1 : Tm n) (e2 : Tm (S n)) (k : Val n), 
+      ifz (succ k) e1 e2 =β e2[k..]
+
+  | BE_letv v e : 
+      let_ (ret v) e =β e[v ..]
+  | BE_ret v1 v2 : 
+      (BV _ v1 v2) -> ret v1 =β ret v2
+  | BE_let e1 e2 e1' e2' : 
+      e1 =β e2 -> e1' =β e2' -> let_ e1 e1' =β let_ e2 e2'
+  | BE_app v1 v2 v1' v2' : 
+      v1 =vβ v2 -> v1' =vβ v2' -> app v1 v1' =β app v2 v2'
+  | BE_ifz v1 v2  e1 e2 e1' e2' : 
+      v1 =vβ v2 -> e1 =β e2 -> e1' =β e2' -> ifz v1 e1 e1' =β ifz v2 e2 e2'
+  | BE_trans e1 e2 e3 : 
+      e1 =β e2 -> e2 =β e3 -> e1 =β e3
+  | BE_sym  e1 e2 : 
+      e1 =β e2 -> e2 =β e1
+with BV (n : nat) : Val n -> Val n -> Prop := 
+  | BV_var x : (var x) =vβ (var x)
+  | BV_unit : unit =vβ unit 
+  | BV_zero : zero =vβ zero
+  | BV_succ v1 v2 : v1 =vβ v2 -> succ v1 =vβ succ v2
+  | BV_abs e1 e2 : e1 =β e2 -> abs e1 =vβ abs e2
+
+
+where "t1 =β t2" := (BE _ t1 t2)
+  and "t1 =vβ t2" := (BV _ t1 t2)
+.
+
+(** * logical equivalence *)
+
+Definition eqtm n e1 e2 := logtm n e1 e2 /\ logtm n e2 e1.
+Definition eqval n v1 v2 := logval n v1 v2 /\ logval n v2 v1.
+
+Instance Compatible_eqtm : Compatible eqtm eqval.
+constructor.
+all: intros.
+all: split.
+all: try match goal with [H : eqval _ _ _ |- _ ] => move: H => [h1 h2] end.
+all: try match goal with [H : eqval _ _ _ |- _ ] => move: H => [h3 h4] end.
+all: try match goal with [H : eqtm _ _ _ |- _ ] => move: H => [h5 h6] end.
+all: try match goal with [H : eqtm _ _ _ |- _ ] => move: H => [h7 h8] end.
+- eapply logvar; eauto.
+- eapply logvar; eauto.
+- eapply logunit; eauto.
+- eapply logunit; eauto.
+- eapply logzero.
+- eapply logzero.
+- eapply logsucc; eauto.
+- eapply logsucc; eauto.
+
+- eapply logabs; eauto.
+- eapply logabs; eauto.
+
+- eapply logret; eauto.
+- eapply logret; eauto.
+- eapply loglet; eauto. 
+- eapply loglet; eauto. 
+- eapply logifz; eauto.
+- eapply logifz; eauto.
+
+- eapply logapp; eauto.
+- eapply logapp; eauto.
+
+Qed.
+
+Instance Reflexive_eqtm : ScopedReflexive eqtm.
+split. eapply scoped_refl. typeclasses eauto.
+eapply scoped_refl. typeclasses eauto.
+Qed.
+
+Instance Reflexive_eqval : ScopedReflexive eqval.
+split. eapply scoped_refl. typeclasses eauto.
+eapply scoped_refl. typeclasses eauto.
+Qed.
+
+Instance Transitive_eqtm : ScopedTransitive eqtm.
+intros ? ? ? ? [h1 h1'][h2 h2']. split.
+  eapply scoped_trans; eauto. 
+  eapply scoped_trans; eauto. 
+Qed.
+
+(** * Beta equivalence implies logical equivalence *)
+
+Fixpoint BE_subrelation n e1 e2 : 
+  BE n e1 e2 -> eqtm n e1 e2
+with BV_subrelation n e1 e2 : 
+  BV n e1 e2 -> eqval n e1 e2.
+Proof.  
+  + intro h. inversion h; subst.
+  - split; eapply CIU_logtm.
+    eapply fun_beta.
+    eapply fun_beta_expand.
+  - split. 
+    eapply CIU_logtm.
+    eapply ifz_zero_beta.
+    eapply CIU_logtm.
+    eapply ifz_zero_beta_expand.
+  - split.
+    eapply CIU_logtm.
+    eapply ifz_succ_beta.
+    eapply CIU_logtm.
+    eapply ifz_succ_beta_expand.
+
+  - split.
+    eapply CIU_logtm.
+    eapply let_ret.
+    eapply CIU_logtm.
+    eapply let_ret_expand.
+  - eapply comp_ret; eauto. 
+  - eapply comp_let; eauto.
+  - eapply comp_app; eauto.
+  - eapply comp_ifz; eauto.
+  - eapply scoped_trans. eapply BE_subrelation. eapply H.
+    eapply BE_subrelation. eapply H0.
+  - apply BE_subrelation in H. destruct H as [h1 h2].
+    split. auto. auto.
+  + intro h. inversion h.
+    eapply val_var; eauto.
+    eapply val_unit; eauto.
+    eapply val_zero; eauto.
+    eapply val_succ; eauto.
+    eapply val_abs; eauto.
+
+Qed.
+
+
+
+
+ 
